SimpLogic-initial.ec
@@ -1,4 +1,6 @@
-(* SimpLogic.ec *)
+(* SimpLogic-initial.ec *)
+
+(* less sophisticated version of SimpLogic.ec *)
 
 prover ["!"].  (* no SMT solvers *)
 
@@ -6,20 +8,33 @@ lemma fa_imp_not_ex_not (P : 'a -> bool) :
   (forall (x : 'a), P x) => ! exists (x : 'a), ! P x.
 proof.
 move => fa_x_P_x.
-case (exists x, ! P x) => [[] x not_P_x | //].
-have // : P x by apply fa_x_P_x.
+case (exists x, ! P x).
+move => ex_x_not_P_x.
+elim ex_x_not_P_x.
+move => x not_P_x.
+have P_x : P x.
+  apply (fa_x_P_x x).
+trivial.
+trivial.
 qed.
 
 lemma not_ex_not_imp_fa (P : 'a -> bool) :
   ! (exists (x : 'a), ! P x) => forall (x : 'a), P x.
 proof.
 move => not_ex_x_not_P_x x.
-case (P x) => [// | not_P_x].
-have // : exists x, ! P x by exists x.
+case (P x).
+trivial.
+move => not_P_x.
+have ex_x_not_P_x : exists (x : 'a), ! P x.
+  exists x.
+  trivial.
+trivial.
 qed.
 
 lemma fa_iff_not_ex_not (P : 'a -> bool) :
   (forall (x : 'a), P x) <=> ! exists (x : 'a), ! P x.
 proof.
-split; [apply fa_imp_not_ex_not | apply not_ex_not_imp_fa].
+split.
+apply fa_imp_not_ex_not.
+apply not_ex_not_imp_fa.
 qed.
