README.md
@@ -16,7 +16,9 @@ First Example: Simple Logic
 
 [`SimpLogic.ec`](../master/SimpLogic.ec) contains the proof of a lemma
 showing how universal quantification can be expressed in terms
-of existential quantification and negation.
+of existential quantification and negation. (The file 
+[`SimpLogic-initial.ec`](../master/SimpLogic-initial.ec) contains
+a less sophisticated precursor to the final, terser proof.)
 
 Second Example: Random Assignment
 --------------------------------------------------------------------
